src/lang/Thread.v
@@ -563,5 +563,75 @@ Module Thread.
     Proof.
       inv STEP. eapply Local.bot_program_step_bot; eauto.
     Qed.
+
+
+    (* step_prev_None *)
+
+    Lemma step_prev_None
+          pf e e1 e2
+          (STEP: step pf e e1 e2):
+      <<PREV: Memory.prev_None e1.(memory) e2.(memory)>>.
+    Proof.
+      inv STEP; inv STEP0; inv LOCAL; ss;
+        try by ii; eapply GET_PREV; eauto.
+      - eapply Memory.promise_prev_None; eauto.
+      - inv LOCAL0. inv WRITE. ss.
+        eapply Memory.promise_prev_None; eauto.
+      - inv LOCAL1. inv LOCAL2. inv WRITE. ss.
+        eapply Memory.promise_prev_None; eauto.
+    Qed.
+
+    Lemma opt_step_prev_None
+          e e1 e2
+          (STEP: opt_step e e1 e2):
+      <<PREV: Memory.prev_None e1.(memory) e2.(memory)>>.
+    Proof.
+      inv STEP; eauto using step_prev_None.
+      ii. eapply GET_PREV; eauto.
+    Qed.
+
+    Lemma rtc_tau_step_prev_None
+          e1 e2
+          (STEPS: rtc tau_step e1 e2):
+      <<PREV: Memory.prev_None e1.(memory) e2.(memory)>>.
+    Proof.
+      induction STEPS.
+      - ii. eapply GET_PREV; eauto.
+      - inv H. inv TSTEP.
+        inv STEP; inv STEP0; inv LOCAL; ss; ii.
+        + exploit Memory.promise_get_from; eauto. i. des.
+          hexploit Memory.promise_prev_None; eauto. i.
+          eapply IHSTEPS; eauto.
+        + inv LOCAL0. inv WRITE.
+          exploit Memory.promise_get_from; eauto. i. des.
+          hexploit Memory.promise_prev_None; eauto. i.
+          eapply IHSTEPS; eauto.
+        + inv LOCAL1. inv LOCAL2. inv WRITE. ss.
+          exploit Memory.promise_get_from; try exact GET; eauto. i. des.
+          hexploit Memory.promise_prev_None; eauto. i.
+          eapply IHSTEPS; eauto.
+    Qed.
+
+    Lemma rtc_all_step_prev_None
+          e1 e2
+          (STEPS: rtc all_step e1 e2):
+      <<PREV: Memory.prev_None e1.(memory) e2.(memory)>>.
+    Proof.
+      induction STEPS.
+      - ii. eapply GET_PREV; eauto.
+      - inv H. inv USTEP.
+        inv STEP; inv STEP0; inv LOCAL; ss; ii.
+        + exploit Memory.promise_get_from; eauto. i. des.
+          hexploit Memory.promise_prev_None; eauto. i.
+          eapply IHSTEPS; eauto.
+        + inv LOCAL0. inv WRITE.
+          exploit Memory.promise_get_from; eauto. i. des.
+          hexploit Memory.promise_prev_None; eauto. i.
+          eapply IHSTEPS; eauto.
+        + inv LOCAL1. inv LOCAL2. inv WRITE. ss.
+          exploit Memory.promise_get_from; try exact GET; eauto. i. des.
+          hexploit Memory.promise_prev_None; eauto. i.
+          eapply IHSTEPS; eauto.
+    Qed.
   End Thread.
 End Thread.
